In our problem, $f(1,t) = 0$.

$f^{\prime}(2, t) = \lambda_1 [1- f(2,t)] \Rightarrow f(2,t) = 1- e^{-\lambda t}$

$f^{\prime}(3, t) = \lambda_1 [1- f(3,t)] + \lambda_2 [2 - f(3,t)] \Rightarrow f(3,t) = \frac{\lambda_1 + 2 \lambda_2}{\lambda_1 + \lambda_2} [1- e^{-(\lambda_1 + \lambda_2) t}]$

$f^{\prime}(3, t) = \lambda_1 [1- f(3,t)] + \lambda_2 [2 - f(3,t)] \Rightarrow f(3,t) = \frac{\lambda_1 + 2 \lambda_2}{\lambda_1 + \lambda_2} [1- e^{-(\lambda_1 + \lambda_2) t}]$

$f^{\prime}(4, t) = \lambda_1 [1 + f(2,t) - f(4,t)] + \lambda_2 [2 - f(4,t)] \Rightarrow f(4,t) = 2- \frac{\lambda_1}{\lambda_2} e^{-\lambda_1 t} - (2- \frac{\lambda_1}{\lambda_2}) e^{-(\lambda_1 + \lambda_2)t}$

$\delta(1,3,t) = 1- f(3,t) = - \frac{\lambda_2}{\lambda_1 + \lambda_2} + \frac{\lambda_1 + 2 \lambda_2}{\lambda_1 + \lambda_2} e^{-(\lambda_1 + \lambda_2)t}$

$\delta(1,4,t) = 1+ f(2,t) - f(4,t) = \frac{\lambda_2- \lambda_1}{\lambda_2} e^{-\lambda_1 t} + (2- \frac{\lambda_1}{\lambda_2}) e^{-(\lambda_1 + \lambda_2)t}$

Critical $t{'}$, when $t < t{'}$, accept $1$.  $\lambda_1 \uparrow, t \uparrow$.

Divide $[0, T]$ into $N$ subintervals to approximate $f(y,t)$:

$f(y,t_{n+1}) = f(y, t_n) + \Delta f(y, t_n)$ with $\Delta f(y, t_n) = f^{'}(y, t_n) \Delta t$, $\Delta t = t_{n+1} - t_{n}$.

Then use $f^{\prime} (y, t_n) = \sum_k \lambda_k \max\{b_k + f(y-w_k, t_n)- f(y, t_n), 0\}$, $f(y, t_{n+1}) = f(y, t_n) + (t_{n+1} - t{n}) f^{\prime}(y, t_n)$ to update.
